Added predicative calculation tactic for ITrees and tidied up some of the relational laws

UTP/ITree_Relation.thy
@@ -8,58 +8,86 @@ text \<open> The relational abstraction captures the possible return values asso
   inputs to a Kleisli tree. It ignores any visible events and treats them as nondeterminism,
   if present. \<close>
 
-definition itree_rel :: "('e, 'a, 'b) ktree \<Rightarrow> ('a \<times> 'b) set" where
-"itree_rel P = {(s, s'). s' \<in> \<^bold>R (P s)}"
+definition itree_pred :: "('e, 'a, 'b) ktree \<Rightarrow> (bool, 'a \<times> 'b) expr" ("\<lbrakk>_\<rbrakk>\<^sub>p") where
+"itree_pred P = (\<lambda> (s, s'). s' \<in> \<^bold>R (P s))"
 
-named_theorems rel
+definition itree_rel :: "('e, 'a, 'b) ktree \<Rightarrow> ('a \<times> 'b) set" where
+"itree_rel P = Collect (itree_pred P)"
+
+lemmas itree_rel_defs = itree_pred_def itree_rel_def
+
+named_theorems itree_pred and itree_rel
 
 definition spec :: "'s scene \<Rightarrow> ('s \<Rightarrow> bool) \<Rightarrow> ('s \<Rightarrow> bool) \<Rightarrow> 's rel" where
 "spec a pre post = {(s, s'). s \<approx>\<^sub>S s' on (- a) \<and> pre s \<longrightarrow> post s'}"
 
-lemma assume_rel [rel]: "itree_rel (assume P) = {(s, s'). s' = s \<and> P s}"
-  apply (auto simp add: itree_rel_def retvals_def assume_def)
+lemma assume_rel [itree_rel]: "itree_rel (assume P) = {(s, s'). s' = s \<and> P s}"
+  apply (auto simp add: itree_rel_defs retvals_def assume_def)
   apply (metis (full_types) Ret_trns diverge_no_Ret_trans itree.inject(1))
   using diverge_no_Ret_trans apply fastforce
   done
 
-lemma test_rel [rel]: "itree_rel (test P) = {(s, s'). s' = s \<and> P s}"
-  apply (auto simp add: itree_rel_def retvals_def test_def)
+lemma test_rel [itree_rel]: "itree_rel (test P) = {(s, s'). s' = s \<and> P s}"
+  apply (auto simp add: itree_rel_defs retvals_def test_def)
   apply (metis (full_types) empty_iff insert_iff retvals_Ret retvals_deadlock retvals_traceI)
   using nonterminates_iff apply force
   done
 
-lemma Skip_rel [rel]: "itree_rel Skip = Id"
-  by (auto simp add: itree_rel_def retvals_def Skip_def)
+lemma Skip_rel [itree_rel]: "itree_rel Skip = Id"
+  by (auto simp add: itree_rel_defs retvals_def Skip_def)
 
-lemma assigns_rel [rel]: "itree_rel \<langle>\<sigma>\<rangle>\<^sub>a = {(s, s'). s' = \<sigma> s}"
-  by (auto simp add: itree_rel_def retvals_def assigns_def)
+lemma assigns_pred [itree_pred]: "\<lbrakk>\<langle>\<sigma>\<rangle>\<^sub>a\<rbrakk>\<^sub>p (s, s') = (s' = \<sigma> s)"
+  by (auto simp add: itree_rel_defs retvals_def assigns_def)
 
-lemma Div_rel [rel]: "itree_rel Div = {}"
-  by (simp add: itree_rel_def)
+lemma assigns_rel [itree_rel]: "itree_rel \<langle>\<sigma>\<rangle>\<^sub>a = {(s, s'). s' = \<sigma> s}"
+  by (simp add: itree_rel_def set_eq_iff assigns_pred)
 
-lemma Stop_rel [rel]: "itree_rel Stop = {}"
-  by (simp add: itree_rel_def)
+lemma Div_rel [itree_rel]: "itree_rel Div = {}"
+  by (simp add: itree_rel_defs)
 
-lemma seq_rel [rel]: "itree_rel (P ;; Q) = itree_rel P O itree_rel Q"
-  by (auto simp add: kleisli_comp_def itree_rel_def relcomp_unfold)
+lemma Stop_pred [itree_pred]: "\<lbrakk>Stop\<rbrakk>\<^sub>p (s, s') = False"
+  by (auto simp add: itree_rel_defs)
 
-lemma cond_rel [rel]: 
+lemma Stop_rel [itree_rel]: "itree_rel Stop = {}"
+  by (simp add: itree_rel_def set_eq_iff Stop_pred)
+
+lemma seq_pred [itree_pred]: "\<lbrakk>P ;; Q\<rbrakk>\<^sub>p (s, s') = (\<exists> s\<^sub>0.  \<lbrakk>P\<rbrakk>\<^sub>p (s, s\<^sub>0) \<and> \<lbrakk>Q\<rbrakk>\<^sub>p (s\<^sub>0, s'))"
+  by (auto simp add: itree_rel_defs kleisli_comp_def)
+
+lemma seq_rel [itree_rel]: "itree_rel (P ;; Q) = itree_rel P O itree_rel Q"
+  by (auto simp add: kleisli_comp_def itree_rel_defs relcomp_unfold)
+
+lemma cond_pred [itree_pred]: 
+  "\<lbrakk>cond_itree C\<^sub>1 B C\<^sub>2\<rbrakk>\<^sub>p (s, s') = (if B s then \<lbrakk>C\<^sub>1\<rbrakk>\<^sub>p (s, s') else \<lbrakk>C\<^sub>2\<rbrakk>\<^sub>p (s, s'))"
+  by (auto simp add: cond_itree_def itree_rel_defs)
+
+lemma cond_rel [itree_rel]: 
   "itree_rel (if B then C\<^sub>1 else C\<^sub>2 fi) 
     = {(s\<^sub>1, s\<^sub>2). if (B s\<^sub>1) then (s\<^sub>1, s\<^sub>2) \<in> itree_rel C\<^sub>1 else (s\<^sub>1, s\<^sub>2) \<in> itree_rel C\<^sub>2}"
-  by (auto simp add: cond_itree_def itree_rel_def)
+  by (auto simp add: cond_itree_def itree_rel_defs)
 
-lemma input_in_where_rel [rel]: 
+lemma input_in_where_rel [itree_rel]: 
   "wb_prism c \<Longrightarrow> itree_rel (input_in_where c A P) = {(s, s'). \<exists> v \<in> A s. fst (P v) s \<and> (s, s') \<in> itree_rel (snd (P v))}" 
-  by (auto simp add: input_in_where_def itree_rel_def retvals_inp_in_where)
+  by (auto simp add: input_in_where_def itree_rel_defs retvals_inp_in_where)
 
-lemma input_in_rel [rel]: 
+lemma input_in_pred [itree_pred]: 
+  "wb_prism c \<Longrightarrow> \<lbrakk>input_in c A P\<rbrakk>\<^sub>p (s, s') = (\<exists> v \<in> A s. \<lbrakk>P v\<rbrakk>\<^sub>p (s, s'))" 
+  by (auto simp add: input_in_where_def itree_rel_defs retvals_inp_in)
+
+lemma input_in_rel [itree_rel]: 
   "wb_prism c \<Longrightarrow> itree_rel (input_in c A P) = {(s, s'). \<exists> v \<in> A s. (s, s') \<in> itree_rel (P v)}" 
-  by (auto simp add: input_in_where_def itree_rel_def retvals_inp_in)
+  by (auto simp add: input_in_where_def itree_rel_defs retvals_inp_in)
 
-lemma input_rel [rel]: "wb_prism c \<Longrightarrow> itree_rel (input c P) = (\<Union> v. itree_rel (P v))"
+lemma input_rel [itree_rel]: "wb_prism c \<Longrightarrow> itree_rel (input c P) = (\<Union> v. itree_rel (P v))"
   by (auto simp add: input_in_rel)
 
-lemma input_in_lit_rel [rel]: "wb_prism c \<Longrightarrow> itree_rel (input_in c (\<guillemotleft>A\<guillemotright>)\<^sub>e P) = (\<Union> v \<in> A. itree_rel (P v))"
+lemma input_in_lit_rel [itree_rel]: "wb_prism c \<Longrightarrow> itree_rel (input_in c (\<guillemotleft>A\<guillemotright>)\<^sub>e P) = (\<Union> v \<in> A. itree_rel (P v))"
   by (auto simp add: input_in_rel)
 
+ML_file \<open>Lens_Rel_Utils.ML\<close>
+
+method rename_rel_alpha_vars = tactic \<open> Lens_Rel_Utils.rename_rel_alpha_vars \<close>
+
+method itree_pred uses add = (expr_simp add: prog_defs itree_pred add; ((rule allI)+)?; rename_rel_alpha_vars)
+                
 end
